Fixed all proofs that didn't survive the previous commit

AlgebraTypes.fst
@@ -1,6 +1,6 @@
 module AlgebraTypes
 
-#push-options "--ifuel 0 --fuel 0 --z3rlimit 1"
+#push-options "--ifuel 0 --fuel 0 --z3rlimit 1 --query_stats"
 
 type binary_op (a:Type) = a -> a -> a
 type unary_op (a:Type) = a -> a
@@ -8,7 +8,7 @@ type predicate (a:Type) = a -> bool
 type binary_relation (a: Type) = a -> a -> bool
 
 let is_reflexive  (#a:Type) (r: binary_relation a) = forall (x:a).     x `r` x
-let is_symmetric  (#a:Type) (r: binary_relation a) = forall (x y:a).   x `r` y           <==> y `r` x
+let is_symmetric  (#a:Type) (r: binary_relation a) = forall (x y:a).   x `r` y == y `r` x
 let is_transitive (#a:Type) (r: binary_relation a) = forall (x y z:a). x `r` y /\ y `r` z ==> x `r` z 
 
 /// We do this for future work with fractions over arbitrary domains.
@@ -25,6 +25,33 @@ type equivalence_wrt (#a: Type) (op: binary_op a) = eq:equivalence_relation a{eq
 let equivalence_is_symmetric (#a:Type) (eq: equivalence_relation a) (x:a) (y:a{x `eq` y})
   : Lemma (x `eq` y == y `eq` x) = ()
 
+private let eq_rel (a:Type) (eq: equivalence_relation a) : (t:equivalence_relation a {t == eq}) = eq
+
+let trans_lemma (#a:Type) (eq: equivalence_relation a) (x y z:a)
+  : Lemma (requires x `eq` y && y `eq` z)  (ensures x `eq` z /\ z `eq` x) = ()
+ 
+let symm_lemma (#a:Type) (eq:equivalence_relation a) (x:a) (y:a) : Lemma (x `eq` y == y `eq` x) = ()
+
+/// FStar does not automatically apply lemmas on equivalence being symmetric reflexive and transitive.
+/// So, I at least make my lemmas such that I care about `eq` operand order as little as possible
+let equivalence_wrt_operation_lemma (#a: Type) (#op: binary_op a) (eq: equivalence_wrt op) (e1 e2 z: a)
+  : Lemma 
+  (requires e1 `eq` e2 \/ e2 `eq` e1) 
+  (ensures 
+    (e1 `op` z) `eq` (e2 `op` z) /\    
+    (e2 `op` z) `eq` (e1 `op` z) /\    
+    (z `op` e1) `eq` (z `op` e2) /\
+    (z `op` e2) `eq` (z `op` e1)) = ()
+    
+let eq_wrt_emulated (#a:Type) (#op: binary_op a) (eq: equivalence_relation a{equivalence_wrt_condition op eq}) (e1 e2 z: a)
+  : Lemma 
+  (requires e1 `eq` e2 \/ e2 `eq` e1) 
+  (ensures 
+    (e1 `op` z) `eq` (e2 `op` z) /\    
+    (e2 `op` z) `eq` (e1 `op` z) /\    
+    (z `op` e1) `eq` (z `op` e2) /\
+    (z `op` e2) `eq` (z `op` e1)) = equivalence_wrt_operation_lemma #a #op eq e1 e2 z
+
 /// Here, we define basic axioms of algebraic structures in form of propositions
 /// about operations and elements. 
 ///
@@ -33,7 +60,10 @@ let equivalence_is_symmetric (#a:Type) (eq: equivalence_relation a) (x:a) (y:a{x
 let is_associative (#a:Type) (op:binary_op a) (eq: equivalence_relation a) = forall (x y z:a). ((x `op` y) `op` z) `eq` (x `op` (y `op` z))
 let is_commutative (#a:Type) (op:binary_op a) (eq: equivalence_relation a) = forall (x y:a). (x `op` y) `eq` (y `op` x)
 
-let associative_operation_lemma (#a:Type) (eq: equivalence_relation a) (op:binary_op a{is_associative op eq}) (x y z:a) : Lemma (((x `op` y) `op` z) `eq` (x `op` (y `op` z)))
+let associative_operation_lemma (#a:Type) (eq: equivalence_relation a) (op:binary_op a{is_associative op eq}) (x y z:a) 
+  : Lemma (
+            ((x `op` y) `op` z) `eq` (x `op` (y `op` z)) && (x `op` (y `op` z)) `eq` ((x `op` y) `op` z)
+          )
   = ()
 
 let commutative_substitution_lemma (#a:Type) (#eq: equivalence_relation a) (op: binary_op a{is_commutative op eq}) 
@@ -57,6 +87,24 @@ let is_invertible_element_of (#a: Type) (op: binary_op a) (eq: equivalence_relat
   = exists (y: a). (is_inverse_element_of op eq neutral x y)
 type neutral_element_of (#a: Type) (op: binary_op a) (eq: equivalence_relation a) = (x:a{is_neutral_of x op eq})
 
+let neutral_lemma (#a:Type) (op: binary_op a) (eq: equivalence_relation a) (x: neutral_element_of op eq) (y:a)
+  : Lemma ((x `op` y) `eq` y /\ (y `op` x) `eq` y) = ()
+
+
+/// If you see something trivial, then it is either here to reduce the rlimit for some bigger lemma,
+/// or a leftover from time where something didn't verify and I made more and more explicit lemmas,
+/// or it should be deleted. I periodically cleanup this file and remove unused lemmas.
+/// Nothing big gets removed anyway.
+
+let neutral_is_unique (#a:Type) (op: binary_op a) (eq: equivalence_wrt op) (u: neutral_element_of op eq) (v: neutral_element_of op eq) : Lemma (eq u v) = ()
+
+let neutral_equivalent_is_neutral (#a:Type) (op: binary_op a) (eq: equivalence_wrt op) (x: neutral_element_of op eq) (y: a{y `eq` x}) : Lemma (is_neutral_of y op eq) =   
+  let aux (t:a) : Lemma (((t `op` y) `eq` t) /\ ((y `op` t) `eq` t)) = equivalence_wrt_operation_lemma eq x y t in
+  FStar.Classical.forall_intro aux;
+  assert (is_neutral_of y op eq);
+  ()
+  
+
 /// The notion of absorbing element, or absorber, is the generalization of integer zero with respect to multiplication
 /// That is, 0x = x0 = 0. Other exmaples are the empty set w.r.t. intersection, 1 w.r.t. GCD in naturals, etc.
 let is_absorber_of (#a:Type) (z:a) (op:binary_op a) (eq: equivalence_relation a) = forall (x:a). ((x `op` z) `eq` z) && ((z `op` x) `eq` z)
@@ -68,10 +116,19 @@ let absorber_lemma (#a:Type) (op:binary_op a) (eq: equivalence_relation a) (z: a
 
 /// Proving that in any magma, there may not be 2 distinct absorbers, is left as an exercise to both Z3 and the reader.
 /// And Z3 is doing fine on that account, just saying.
-let absorber_is_unique (#a:Type) (op: binary_op a) (eq: equivalence_relation a) (z1 z2: absorber_of op eq) : Lemma (eq z1 z2) = ()
+let absorber_is_unique (#a:Type) (op: binary_op a) (eq: equivalence_relation a) (z1 z2: a) : Lemma (requires is_absorber_of z1 op eq /\ is_absorber_of z2 op eq) (ensures eq z1 z2 /\ eq z2 z1) = ()
 
-let absorber_eq_is_also_absorber (#a:Type) (op: binary_op a) (eq: equivalence_wrt op) (absorber: absorber_of op eq)
-(other:a{eq other absorber}) : Lemma (is_absorber_of other op eq) = ()
+let absorber_eq_is_abs (#a:Type) (op: binary_op a) (eq: equivalence_wrt op) (z1: absorber_of op eq) (z2: a{z2 `eq` z1}) (t: a) : Lemma (t `op` z2 `eq` z2 /\ z2 `op` t `eq` z2) = equivalence_wrt_operation_lemma eq z1 z2 t 
+
+let absorber_equal_is_absorber (#a:Type) (op:binary_op a) (eq: equivalence_wrt op) (z1: absorber_of op eq) (z2:a{z2 `eq` z1}) : Lemma (is_absorber_of z2 op eq) = 
+  FStar.Classical.forall_intro (absorber_eq_is_abs op eq z1 z2)
+
+let absorber_equal_is_absorber_req (#a:Type) (op: binary_op a) (eq: equivalence_wrt op) (z1 z2: a) 
+  : Lemma (requires is_absorber_of z1 op eq /\ eq z1 z2) (ensures is_absorber_of z2 op eq) = absorber_equal_is_absorber op eq z1 z2
+  
+let nonabsorber_equal_is_nonabsorber (#a:Type) (op: binary_op a) (eq: equivalence_wrt op) (p: non_absorber_of op eq) (q:a{q `eq` p}) : Lemma (~(is_absorber_of q op eq)) 
+  = (Classical.move_requires (absorber_equal_is_absorber_req op eq q)) p
+
 
 /// Since we are using custom equivalence relation, we specifically assure the existence of
 /// the unit. We also write "forall" since, for example, for fractions, there'll also be neutral
@@ -81,22 +138,111 @@ let absorber_eq_is_also_absorber (#a:Type) (op: binary_op a) (eq: equivalence_wr
 /// For arbitrary domains, there is no hope of reduced fractions, so the notions for inverses and neutrals
 /// stays in its most general form.
 let is_inverse_operation_for (#a: Type) (inv: unary_op a) (op: binary_op a) (eq: equivalence_relation a) 
-  = (exists (at_least_one_neutral: a). is_neutral_of at_least_one_neutral op eq) /\
-    (forall (u: neutral_element_of op eq) (x: a). ((x `op` (inv x)) `eq` u) /\ (((inv x) `op` x) `eq` u))
+  = (forall (x:a). is_neutral_of (op x (inv x)) op eq /\ is_neutral_of (op (inv x) x) op eq)
+
+let inverse_operation_lemma (#a:Type) (op: binary_op a) (eq: equivalence_wrt op) (inv: unary_op a{is_inverse_operation_for inv op eq}) (x: a) : Lemma (is_neutral_of (x `op` (inv x)) op eq) = ()
+
 
 /// The inverse operation type is also a refinement for arbitrary unary operation 
 type inverse_op_for (#a: Type) (op: binary_op a) (eq: equivalence_relation a) 
   = (inv:unary_op a{is_inverse_operation_for inv op eq})
 
+let inverses_produce_neutral (#a:Type) (eq: equivalence_relation a) (op: binary_op a{is_associative op eq /\ equivalence_wrt_condition op eq}) (inv: inverse_op_for op eq) (x y: a)
+  : Lemma (requires inv x `eq` y)
+          (ensures is_neutral_of (x `op` y) op eq) =
+   // assert_spinoff ((inv x `eq` y));
+ //   assert (is_neutral_of (x `op` inv x) op eq);
+    equivalence_wrt_operation_lemma #a #op eq (inv x) y x;
+  //  assert (x `op` y `eq` (x `op` inv x));
+    neutral_equivalent_is_neutral op eq (x `op` inv x) (x `op` y)
+
+let group_operation_lemma (#a:Type) (eq: equivalence_relation a) 
+                             (op: binary_op a{is_associative op eq /\ equivalence_wrt_condition op eq}) 
+                             (inv: inverse_op_for op eq) (x y z:a) 
+  : Lemma (requires (x `op` z) `eq` (y `op` z)) (ensures (x `eq` y)) = 
+  let z'  = inv z in
+  let op = op in
+  let eq : equivalence_wrt op = eq in
+  let zz' = z `op` z' in
+  let xz = x `op` z in                         // suppose zz'    = 0 (always possible in a group)
+  let yz = y `op` z in                         // we have xz     = yz
+  equivalence_wrt_operation_lemma eq xz yz z'; // then,   (xz)z' = (yz)z'
+  associative_operation_lemma eq op x z z';    // or,     x(zz') = (yz)z'
+  neutral_lemma op eq zz' x;                   // zz'=0,   (zz') = x
+  trans_lemma eq (xz `op` z') (x `op` zz') x;  // transitivity, (xz)z' = x(zz') = x, (xz)z'=x
+  trans_lemma eq x (xz `op` z') (yz `op` z');  // transitivity, x = (xz)z' = (yz)z'
+  associative_operation_lemma eq op y z z';    // assoc again, (yz)z' = y(zz') 
+  neutral_lemma op eq zz' y;                   // neutral again, y(zz')=y.
+  ()                                           // the rest is left as an exercise for Z3
+
+ 
+#push-options "--ifuel 0 --fuel 0 --z3rlimit 2"
+let producing_neutral_means_inverses (#a:Type) (eq: equivalence_relation a) (op: binary_op a{is_associative op eq /\ equivalence_wrt_condition op eq}) (inv: inverse_op_for op eq) (x y: a)
+  : Lemma (requires is_neutral_of (x `op` y) op eq) (ensures inv x `eq` y)  = 
+  
+  assert (is_neutral_of (inv y `op` y) op eq);
+//  assert (is_neutral_of (x `op` y) op eq);
+  neutral_is_unique op eq  (inv y `op` y) (x `op` y);
+  group_operation_lemma eq op inv (inv y) x y;
+//  assert (inv y `eq` x);
+  equivalence_wrt_operation_lemma #a #op eq (inv y) x y;
+  equivalence_wrt_operation_lemma #a #op eq (y `op` inv y) (y `op` x) (inv x);  
+//  assert (((y `op` inv y) `op` inv x) `eq` ((y `op` x) `op` (inv x)));
+//  assert (is_neutral_of (y `op` inv y) op eq);
+  neutral_lemma op eq (y `op` inv y) (inv x);
+//  assert ((inv x) `eq` ((y `op` x) `op` (inv x)));
+  associative_operation_lemma eq op y x (inv x);
+//  assert ((inv x) `eq` (y `op` (x `op` inv x)));
+  neutral_lemma op eq (x `op` inv x) y;
+  trans_lemma eq (inv x) (y `op` (x `op` inv x)) y;
+//  assert (inv x `eq` y);
+//  assert_spinoff (inv x `eq` y == true);
+  ()
+#pop-options
+
+let equivalence_lemma_from_implications (#a:Type) (p) (q)
+                                        (to_right : (x:a)->(y:a)->Lemma (requires p x y) (ensures q x y))
+                                        (to_left  : (x:a)->(y:a)->Lemma (requires q x y) (ensures p x y))
+                                        (x:a) (y:a)
+                                        : Lemma (p x y <==> q x y) = 
+                                        (Classical.move_requires_2 to_right) x y;
+                                        (Classical.move_requires_2 to_left) x y
+ 
+(*
+let inverses_produce_neutral (#a:Type) (eq: equivalence_relation a) (op: binary_op a{is_associative op eq /\ equivalence_wrt_condition op eq}) (inv: inverse_op_for op eq) (x y: a)
+  : Lemma (requires (inv x `eq` y))
+          (ensures is_neutral_of (x `op` y) op eq) =
+*)
+
+#push-options "--ifuel 0 --fuel 0 --z3rlimit 14"
+  let inverse_lemma_def (#a:Type) (eq: equivalence_relation a) (op: binary_op a{is_associative op eq /\ equivalence_wrt_condition op eq}) (inv: inverse_op_for op eq) (x y: a)
+  : Lemma (is_neutral_of (x `op` y) op eq <==> inv x `eq` y) = 
+  (FStar.Classical.move_requires_2 (inverses_produce_neutral eq op inv)) x y;
+  (FStar.Classical.move_requires_2 (producing_neutral_means_inverses eq op inv)) x y;
+  assert (is_neutral_of (op x y) op eq ==> inv x `eq` y);   
+  () 
+#pop-options
+
+ 
+
 /// We shall generally keep in mind that distributivity laws must be considered separately
 /// If in future we consider K[x] with multiplication f(x)*g(x) defined as composition f(g(x)),
 /// we will do well to remember that only one of the two distributivities holds there.
-let is_right_distributive (#a:Type) (op_mul:binary_op a) (op_add:binary_op a) (eq: equivalence_relation a) =
-  forall (x y z:a). (x `op_mul` (y `op_add` z)) `eq` ((x `op_mul` y) `op_add` (x `op_mul` z))
 let is_left_distributive (#a:Type) (op_mul:binary_op a) (op_add:binary_op a) (eq: equivalence_relation a) =
+  forall (x y z:a). (x `op_mul` (y `op_add` z)) `eq` ((x `op_mul` y) `op_add` (x `op_mul` z))
+let is_right_distributive (#a:Type) (op_mul:binary_op a) (op_add:binary_op a) (eq: equivalence_relation a) =
   forall (x y z:a). ((x `op_add` y) `op_mul` z) `eq` ((x `op_mul` z) `op_add` (y `op_mul` z))
 let is_fully_distributive (#a:Type) (op_mul:binary_op a) (op_add:binary_op a) (eq: equivalence_relation a) =
-  (is_right_distributive op_mul op_add eq) /\ (is_left_distributive op_mul op_add eq) 
+  forall (x y z:a). ((x `op_mul` (y `op_add` z)) `eq` ((x `op_mul` y) `op_add` (x `op_mul` z))) /\ (((x `op_add` y) `op_mul` z) `eq` ((x `op_mul` z) `op_add` (y `op_mul` z)))
+
+let fully_distributive_is_both_left_and_right  (#a:Type) (op_mul:binary_op a) (op_add:binary_op a) (eq: equivalence_relation a) 
+  : Lemma (is_fully_distributive op_mul op_add eq <==> is_left_distributive op_mul op_add eq /\ is_right_distributive op_mul op_add eq) = ()
+
+let left_distributivity_lemma (#a:Type) (op_mul:binary_op a) (op_add:binary_op a) (eq: equivalence_relation a) (x y z: a)
+  : Lemma (requires is_left_distributive op_mul op_add eq) (ensures (x `op_mul` (y `op_add` z)) `eq` ((x `op_mul` y) `op_add` (x `op_mul` z))) = ()
+
+let right_distributivity_lemma (#a:Type) (op_mul:binary_op a) (op_add:binary_op a) (eq: equivalence_relation a) (x y z: a)
+  : Lemma (requires is_right_distributive op_mul op_add eq) (ensures ((x `op_add` y) `op_mul` z) `eq` ((x `op_mul` z) `op_add` (y `op_mul` z))) = ()
 
 /// Domain defining property (the alternative form is the Cancellation Law, (ax=bx ==> (x=0 \/ a=b)
 let has_no_zero_divisors (#a:Type) (zero:a) (op_mul: binary_op a) (eq: equivalence_relation a)=
@@ -152,6 +298,9 @@ noeq type magma (#a: Type) =
   inv: (t:unary_op a{ respects_equivalence t eq });
   neutral: a
 }
+
+//let magma_equality_is_symmetric (#a:Type) (m: magma #a) (x y:a) : Lemma (x `m.eq` y == y `m.eq` x) [SMTPat(x `m.eq` y)] = symm_lemma m.eq x y
+
 type semigroup (#a:Type)             = g: magma #a{is_associative g.op g.eq}
 type commutative_magma (#a:Type)     = g: magma #a{is_commutative g.op g.eq}
 type commutative_semigroup (#a:Type) = g: semigroup #a{is_commutative g.op g.eq}
@@ -160,71 +309,59 @@ type commutative_monoid (#a:Type)    = g: monoid #a{is_commutative g.op g.eq}
 type group (#a:Type)                 = g: monoid #a{is_inverse_operation_for g.inv g.op g.eq}
 type commutative_group (#a:Type)     = g: group #a{is_commutative g.op g.eq}
 
+let magma_eq_wrt_condition (#a:Type) (m: magma #a) : Lemma(equivalence_wrt_condition m.op m.eq) = ()
+
+let absorber_never_equals_non_absorber (#a: Type) (op: binary_op a) (eq: equivalence_wrt op) 
+  (x: absorber_of op eq) (y: non_absorber_of op eq) : Lemma (~(x `eq` y)) = 
+  if (x `eq` y) then absorber_equal_is_absorber op eq x y
+
+let plus_associative 
+  (#a:Type) 
+  (op: binary_op a) 
+  (eq: equivalence_wrt op)  
+  (x y z: a)
+  : Lemma
+  (requires is_associative op eq)
+  (ensures  ((x `op` y) `op` z) `eq` (x `op` (y `op` z))) = ()
+
 let is_absorber_of_magma (#a:Type) (z: a) (m: magma #a) = is_absorber_of z m.op m.eq
-
-/// If you see something trivial, then it is either here to reduce the rlimit for some bigger lemma,
-/// or a leftover from time where something didn't verify and I made more and more explicit lemmas,
-/// or it should be deleted. I periodically cleanup this file and remove unused lemmas.
-/// Nothing big gets removed anyway.
-
-let neutral_is_unique (#a:Type) (g: semigroup #a) (u: neutral_element_of g.op g.eq) (v: neutral_element_of g.op g.eq) : Lemma (g.eq u v) = ()
-
-let neutral_equivalent_is_neutral (#a:Type) (op: binary_op a) (eq: equivalence_wrt op ) (x: neutral_element_of op eq) (y: a{y `eq` x}) : Lemma (is_neutral_of y op eq) = 
-  let aux_right (t: a) : Lemma ((t `op` y) `eq` t) = 
-    assert (y `eq` x);
-    assert (forall (p q r:a). (p `eq` q) <==> ((p `op` r) `eq` (q `op` r)));
-    assert (t `op` x `eq` t);
-    assert ((t `op` y) `eq` (t `op` x));
-    assert ((t `op` y) `eq` t);
-    () in
-  let aux_left (t: a) : Lemma ((y `op` t) `eq` t) = 
-    assert (y `eq` x);
-    assert (forall (p q r:a). (p `eq` q) <==> ((r `op` p) `eq` (r `op` q)));
-    assert (x `op` t `eq` t);
-    assert ((y `op` t) `eq` (x `op` t));
-    assert ((y `op` t) `eq` t);
-    () in
-  FStar.Classical.forall_intro aux_left;
-  FStar.Classical.forall_intro aux_right;
-  assert (is_neutral_of y op eq);
-  ()
-/// FStar does not automatically apply lemmas on equivalence being symmetric reflexive and transitive.
-/// So, I at least make my lemmas such that I care about `eq` operand order as little as possible
-let equivalence_wrt_operation_lemma (#a: Type) (#op: binary_op a) (eq: equivalence_wrt op) (e1 e2 z: a)
-  : Lemma 
-  (requires e1 `eq` e2 \/ e2 `eq` e1) 
-  (ensures 
-    (e1 `op` z) `eq` (e2 `op` z) /\    
-    (e2 `op` z) `eq` (e1 `op` z) /\    
-    (z `op` e1) `eq` (z `op` e2) /\
-    (z `op` e2) `eq` (z `op` e1)) = ()
-let equivalence_wrt_operation_lemma_inverse (#a: Type) (#op: binary_op a) (eq: equivalence_wrt op) (e1 e2 z: a)
-  : Lemma 
-  (requires 
-    ((e1 `op` z) `eq` (e2 `op` z) \/ (e2 `op` z) `eq` (e1 `op` z)) /\ 
-    ((z `op` e1) `eq` (z `op` e2) \/ (z `op` e2) `eq` (z `op` e1))) 
-  (ensures e1 `eq` e2 /\ e2 `eq` e1) = ()
-let equivalence_wrt_operation_lemma_twoway (#a: Type) (#op: binary_op a) (eq: equivalence_wrt op) (e1 e2 z: a)
-  : Lemma ((e1 `op` z) `eq` (e2 `op` z) /\    
-           (e2 `op` z) `eq` (e1 `op` z) /\    
-           (z `op` e1) `eq` (z `op` e2) /\
-           (z `op` e2) `eq` (z `op` e1)
-           <==> 
-            e1 `eq` e2 /\ e2 `eq` e1) = ()
-
-let eq_wrt_emulated (#a:Type) (#op: binary_op a) (eq: equivalence_relation a{equivalence_wrt_condition op eq}) (e1 e2 z: a)
-  : Lemma 
-  (requires e1 `eq` e2 \/ e2 `eq` e1) 
-  (ensures 
-    (e1 `op` z) `eq` (e2 `op` z) /\    
-    (e2 `op` z) `eq` (e1 `op` z) /\    
-    (z `op` e1) `eq` (z `op` e2) /\
-    (z `op` e2) `eq` (z `op` e1)) = equivalence_wrt_operation_lemma #a #op eq e1 e2 z
 
 /// When I try to keep the rlimit at minimum, lemmas like this one sometimes help
 let neutral_inverse_is_neutral (#a:Type) (g: group #a) : Lemma (g.neutral `g.eq` (g.inv g.neutral)) =  
   assert ((g.neutral `g.op` (g.inv g.neutral)) `g.eq` g.neutral)
 
+let group_op_lemma (#a:Type) (g: group #a) (x y z:a) 
+  : Lemma (requires (x `g.op` z) `g.eq` (y `g.op` z)) (ensures (x `g.eq` y)) = group_operation_lemma g.eq g.op g.inv x y z
+ 
+let flip_lemma p1 p2 (q:unit -> Lemma (requires p1) (ensures p2))
+  : Lemma (requires ~p2) (ensures ~p1)
+  = FStar.Classical.move_requires q ()
+
+#push-options "--ifuel 0 --fuel 0 --z3rlimit 4 --query_stats"
+let absorber_for_invertible_operation_is_nonsense (#a:Type) (op: binary_op a) (eq: equivalence_wrt op) (inv: inverse_op_for op eq)
+   (y: non_absorber_of op eq) (z:a) : Lemma (requires is_absorber_of z op eq) (ensures False) =  
+    absorber_never_equals_non_absorber op eq z y;
+    let z' = inv z in
+    let zz' = op z (inv z) in
+    let yzz' = op y zz' in                                // I write "the absorber" here to underline its uniqueness
+    absorber_lemma op eq z z';                        (** 1. By definition of absorber, zz' should be equal to z.      *)
+    absorber_equal_is_absorber op eq z zz';           (** 2. Any element equal to an absorber is the absorber,         *)
+                                                      (**    therefore, zz' is also the absorber, since zz' = z.       *)
+    (* assert (is_neutral_of zz' op eq); *)           (** 3. By definition of inverse, zz' is the neutral element.     *)
+    (* assert (yzz' `eq` y);             *)           (** 4. By definition of neutral element (zz'), yzz' = y          *)
+                                                      (**    This assertion somehow slows down the prover a lot!       *)
+    (* assert (yzz' `eq` zz');           *)           (** 5. But as zz' is the absorber, yzz' = zz'!                   *)
+    absorber_equal_is_absorber op eq zz' yzz';        (** 6. Being equal to the absorber zz', yzz' is the absorber     *)
+    nonabsorber_equal_is_nonabsorber op eq y yzz';    (** 7. But, as an equal of y, yzz' can't be an absorber!         *)
+    assert_spinoff (~(is_absorber_of yzz' op eq));    (**    So, we got the contradiction here!                        *)
+    assert_spinoff (is_absorber_of yzz' op eq);       (**    Deleting the last two asserts gives 10x proof slowdown!   *)
+    ()
+#pop-options 
+
+let group_has_no_absorbers (#a:Type) (g: group #a) (z:a) (y:non_absorber_of g.op g.eq) 
+  : Lemma (~(is_absorber_of z g.op g.eq)) = 
+  (Classical.move_requires (absorber_for_invertible_operation_is_nonsense g.op g.eq g.inv y)) z
+ 
 /// In our pursuit of sanity, we only consider ring-like structures that are at least rigs,
 /// with addition forming a commutative group, and multiplication forming a semigroup that
 /// is fully (left and right) distributive over addition
@@ -241,9 +378,12 @@ let nat_function_value (#a:Type) (op: binary_op a) (eq: equivalence_relation a) 
 
 let has_no_absorber_divisors (#a:Type) (op: binary_op a) (eq: equivalence_relation a) = forall (x y: a). is_absorber_of (op x y) op eq <==> (is_absorber_of x op eq) \/ (is_absorber_of y op eq)
 
-let domain_multiplication_law (#a:Type) (eq: equivalence_relation a) (mul: binary_op a{has_no_absorber_divisors mul eq}) (x y: non_absorber_of mul eq)
-  : Lemma ( ~ (is_absorber_of (mul x y) mul eq) ) = ()
+let domain_multiplication_law (#a:Type) (eq: equivalence_relation a) (mul: binary_op a{has_no_absorber_divisors mul eq}) (x y: a)
+  : Lemma (~(is_absorber_of x mul eq) /\ ~(is_absorber_of y mul eq) <==> ~ (is_absorber_of (mul x y) mul eq)) = ()
  
+let domain_multiplication_law_inv (#a:Type) (eq: equivalence_relation a) (mul: binary_op a{has_no_absorber_divisors mul eq}) (x y: a)
+  : Lemma ((is_absorber_of x mul eq) \/ (is_absorber_of y mul eq) <==> (is_absorber_of (mul x y) mul eq)) = ()
+  
 let euclidean_norm_property (#a:Type) (eq: equivalence_relation a) (mul: binary_op a{has_no_absorber_divisors mul eq}) (x y: non_absorber_of mul eq) (f: nat_function_defined_on_non_absorbers mul eq) = 
   domain_multiplication_law eq mul x y;
   nat_function_value mul eq f (mul x y) >= nat_function_value mul eq f x 
@@ -312,7 +452,6 @@ let is_normal_part_function (#a:Type) (#mul: binary_op a) (#eq: equivalence_wrt 
 type normal_part_function (#a: Type) (#mul: binary_op a) (#eq: equivalence_wrt mul) (unit_part_func: a -> a)
   = f:(a -> (unit_normals_of mul eq unit_part_func)){ is_normal_part_function unit_part_func f }
 
-
 let unit_part_func_of_product_is_product_of_unit_parts (#a: Type) (#mul: binary_op a) (#eq: equivalence_wrt mul)
   (unit_part_func: unit_part_function mul eq) (x y: non_absorber_of mul eq) 
   : Lemma((unit_part_func (x `mul` y)) `eq` ((unit_part_func x) `mul` (unit_part_func y))) = 
@@ -332,7 +471,7 @@ let product_of_unit_normals_is_normal (#a: Type) (#mul: binary_op a) (#eq: equiv
 
 type test_unit_part_func (#a: Type) (mul: binary_op a) (eq: equivalence_wrt mul) = unit_part_function mul eq
 
-#push-options "--ifuel 0 --fuel 0 --z3rlimit 3"
+#push-options "--ifuel 0 --fuel 0 --z3rlimit 4"
 noeq type ring (#a: Type) = {
   addition: commutative_group #a;
 
@@ -351,6 +490,222 @@ noeq type ring (#a: Type) = {
   normal_part_of: a -> unit_normals_of multiplication.op eq unit_part_of;
   euclidean_norm: nat_function_defined_on_non_absorbers multiplication.op eq 
 }
+#pop-options
+
+
+#push-options "--ifuel 0 --fuel 0 --z3rlimit 3"
+let ring_addition_neutral_is_unique (#a:Type) (r:ring #a) (n: a{is_neutral_of n r.addition.op r.eq}) 
+  : Lemma (r.eq n r.addition.neutral && r.eq r.addition.neutral n)[SMTPat(is_neutral_of n r.addition.op r.eq)] = ()
+#pop-options
+
+let neg_of (#a:Type) (r: ring #a) (p:a) : (t:a{ t `r.eq` (r.addition.neutral `r.addition.op` (r.addition.inv p) )}) = r.addition.inv p
+
+let minus_of (#a:Type) (r: ring #a) (x:a) (y:a) : (t:a{ t `r.eq` (x `r.addition.op` (r.addition.inv y) )}) = x `r.addition.op` (neg_of r y)
+
+let minus_minus_x_is_x (#a:Type) (r: ring #a) (x: a) : Lemma (neg_of r (neg_of r x) `r.eq` x /\ x `r.eq` (neg_of r (neg_of r x))) = 
+//  assert (r.addition.op x (neg_of r x) `r.eq` r.addition.neutral);
+//  assert (r.addition.op (neg_of r (neg_of r x)) (neg_of r x) `r.eq` r.addition.neutral);
+//  trans_lemma r.eq (r.addition.op x (neg_of r x)) r.addition.neutral (r.addition.op (neg_of r (neg_of r x)) (neg_of r x));
+//  assert ((r.addition.op x (neg_of r x)) `r.eq` (r.addition.op (neg_of r (neg_of r x)) (neg_of r x))); 
+  group_op_lemma r.addition x (neg_of r (neg_of r x)) (neg_of r x);  
+  ()
+ 
+#push-options "--ifuel 2 --fuel 0 --z3rlimit 4"
+let ring_additive_inv_x_is_x_times_minus_one (#a:Type) (r: ring #a) (x: a)
+  : Lemma ((r.addition.inv x) `r.eq` (r.multiplication.op x (r.addition.inv r.multiplication.neutral)) /\
+           (r.multiplication.op x (r.addition.inv r.multiplication.neutral)) `r.eq` (r.addition.inv x)) = 
+    let eq = r.eq in
+    let mul = r.multiplication.op in
+    let add = r.addition.op in
+    let inv = r.addition.inv in 
+    let zero = r.addition.neutral in
+    let one = r.multiplication.neutral in
+    let ix = inv x in  
+    assert (is_neutral_of (one `add` (inv one)) add eq);
+    neutral_is_unique r.addition.op r.eq zero (one `add` (inv one));
+//    assert (zero `eq` (one `add` (inv one)));
+    equivalence_wrt_operation_lemma #a #mul eq zero (one `add` (inv one)) x;
+//    assert (mul x (one `add` (inv one)) `eq` (mul x zero));
+//    assert (mul x zero `eq` zero);
+//    assert ((mul x (one `add` (inv one))) `eq` ((mul x one) `add` (mul x (inv one)))); 
+    symm_lemma eq ((mul x one) `add` (mul x (inv one))) (mul x (one `add` (inv one)));
+    //this one speeds up the process if uncommented
+    assert_spinoff (((mul x one) `add` (mul x (inv one))) `eq` (mul x (one `add` (inv one))));    
+    //this one requires spinoff!!! for some reason...
+    assert_spinoff (mul x (one `add` (inv one)) `eq` zero);       
+    trans_lemma eq ((mul x one) `add` (mul x (inv one))) (mul x (one `add` (inv one))) zero;
+    assert (((mul x one) `add` (mul x (inv one))) `eq` zero);
+    assert (is_neutral_of zero add eq);
+    neutral_equivalent_is_neutral add eq zero ((mul x one) `add` (mul x (inv one)));
+    assert (is_neutral_of ((mul x one) `add` (mul x (inv one))) add eq);
+    producing_neutral_means_inverses eq add inv (mul x one) (mul x (inv one));
+    assert (eq (inv (mul x one)) (mul x (inv one)));
+    assert (is_neutral_of one mul eq);
+    neutral_lemma mul eq one x;
+    assert (mul x one `eq` x);    
+    assert (inv (mul x one) `eq` (inv x));
+    trans_lemma eq (inv x) (inv (mul x one)) (mul x (inv one));
+  ()
+#pop-options
+
+let equal_elements_means_equal_inverses (#a:Type) (r: ring #a) (x y:a) 
+  : Lemma (r.eq x y == (r.addition.inv x `r.eq` r.addition.inv y) /\ r.eq x y == (r.addition.inv y `r.eq` r.addition.inv x)) = 
+  let one = r.multiplication.neutral in
+  let add = r.addition.op in
+  let mul = r.multiplication.op in
+  let eq = r.eq in
+  let neg = r.addition.inv in
+  if (x `eq` y) then (()) else (
+    if ( (neg x) `eq` (neg y) ) then (
+      equivalence_wrt_operation_lemma #a #r.multiplication.op r.eq (neg x) (neg y) (neg one);      
+      assert (r.multiplication.op (neg x) (neg one) `r.eq` r.multiplication.op (neg y) (neg one));      
+      ring_additive_inv_x_is_x_times_minus_one r (neg x);
+      assert (r.eq (neg (neg x)) (r.multiplication.op (neg x) (neg one)));
+      minus_minus_x_is_x r x;
+      trans_lemma eq x (neg (neg x)) (r.multiplication.op (neg x) (neg one));
+
+      assert (x `r.eq` (r.multiplication.op (neg x) (neg one)));
+      assert ((neg x `mul` neg one) `eq` (neg y `mul` neg one));
+      assert ((neg x `mul` neg one) `eq` x);
+      ring_additive_inv_x_is_x_times_minus_one r (neg y);
+      minus_minus_x_is_x r y;
+      trans_lemma eq y (neg (neg y)) (r.multiplication.op (neg y) (neg one)); 
+      assert (eq (neg y `mul` neg one) y);
+      trans_lemma eq x (neg x `mul` neg one) (neg y `mul` neg one);
+      trans_lemma eq x (neg y `mul` neg one) y;
+      ()
+    ) else ()
+  )  
+ 
+let inv_switch_lemma (#a:Type) (r: ring #a) (x y:a) : Lemma (x `r.eq` (r.addition.inv y) <==> (r.addition.inv x) `r.eq` y) =   
+  if (x `r.eq` r.addition.inv y) then (
+    equal_elements_means_equal_inverses r x (r.addition.inv y);
+    minus_minus_x_is_x r y;
+    trans_lemma r.eq (r.addition.inv x) (r.addition.inv (r.addition.inv y)) y;
+    ()
+  )
+  else if (r.addition.inv x `r.eq` y) then (
+    equal_elements_means_equal_inverses r (r.addition.inv x) y;
+    minus_minus_x_is_x r x;    
+    trans_lemma r.eq x (r.addition.inv (r.addition.inv x)) (r.addition.inv y);
+    ()
+  ) else ()
+
+let ring_additive_inverse_is_unique (#a:Type) (r:ring #a) (x y: a) 
+  : Lemma (requires x `r.eq` y \/ y `r.eq` x) 
+          (ensures r.addition.inv x `r.eq` r.addition.inv y /\ r.addition.inv y `r.eq` r.addition.inv x) 
+  = ()
+
+#push-options "--ifuel 1 --fuel 0 --z3rlimit 1"
+let ring_additive_inv_x_is_minus_one_times_x (#a:Type) (r: ring #a) (x: a)
+  : Lemma ((r.addition.inv x) `r.eq` (r.multiplication.op (r.addition.inv r.multiplication.neutral) x)) = 
+    let eq = r.eq in
+    let mul = r.multiplication.op in
+    let add = r.addition.op in
+    let inv = r.addition.inv in 
+    let zero = r.addition.neutral in
+    let one = r.multiplication.neutral in
+    let ix = inv x in  
+    assert (is_neutral_of (inv one `add` one) add eq);
+    neutral_is_unique r.addition.op r.eq zero (inv one `add` one);
+    equivalence_wrt_operation_lemma #a #mul eq zero (inv one `add` one) x;
+//    assert (mul (inv one `add` one) x `eq` (mul (inv one) x `add` mul one x));
+    symm_lemma eq (mul (inv one) x `add` mul one x) (mul (inv one `add` one) x);
+//    assert ( (mul (inv one) x `add` mul one x) `eq` (mul (inv one `add` one) x));
+    
+    assert_spinoff (mul (inv one `add` one) x `eq` zero);
+    trans_lemma eq (mul (inv one) x `add` mul one x) (mul (inv one `add` one) x) zero;
+//  assert ((mul (inv one) x `add` mul one x) `eq` zero);
+    neutral_equivalent_is_neutral add eq zero (mul (inv one) x `add` mul one x);
+    producing_neutral_means_inverses eq add inv (mul (inv one) x) (mul one x);
+//    assert (inv (mul (inv one) x) `eq` (mul one x));
+    inv_switch_lemma r (mul (inv one) x) (mul one x);
+//    assert (mul (inv one) x `eq` (inv (mul one x)));
+    symm_lemma eq (inv (mul one x)) (mul (inv one) x);
+//    assert (mul one x `eq` x);
+    ring_additive_inverse_is_unique r x (mul one x);
+//    assert (inv x `eq` inv (mul one x));
+//    assert (inv (mul one x) `eq` mul (inv one) x);
+    trans_lemma eq (inv x) (inv (mul one x)) (mul (inv one) x);    
+  ()
+#pop-options
+
+let ring_times_minus_one_is_commutative (#a:Type) (r: ring #a) (x:a) 
+  : Lemma ( 
+            (x `r.multiplication.op` r.addition.inv r.multiplication.neutral) `r.eq` (r.addition.inv r.multiplication.neutral `r.multiplication.op` x) &&
+            (x `r.multiplication.op` r.addition.inv r.multiplication.neutral) `r.eq` (r.addition.inv x) &&
+            (r.addition.inv x) `r.eq` (x `r.multiplication.op` r.addition.inv r.multiplication.neutral) &&
+            (r.addition.inv x) `r.eq` (r.addition.inv r.multiplication.neutral `r.multiplication.op` x) &&
+            (r.addition.inv r.multiplication.neutral `r.multiplication.op` x) `r.eq` (x `r.multiplication.op` r.addition.inv r.multiplication.neutral) &&
+            (r.addition.inv r.multiplication.neutral `r.multiplication.op` x) `r.eq` (r.addition.inv x)
+          ) = 
+  ring_additive_inv_x_is_minus_one_times_x r x;
+  ring_additive_inv_x_is_x_times_minus_one r x
+
+let ring_x_times_minus_y_is_minus_xy (#a:Type) (r:ring #a) (x y: a) : Lemma ((x `r.multiplication.op` r.addition.inv y) `r.eq` (r.addition.inv (x `r.multiplication.op` y))) =   
+  ring_additive_inv_x_is_x_times_minus_one r y;
+  let eq = r.eq in
+  let mul = r.multiplication.op in
+  let add = r.addition.op in
+  let neg = r.addition.inv in 
+  let zero = r.addition.neutral in
+  let one = r.multiplication.neutral in
+  ring_additive_inv_x_is_x_times_minus_one r y; // -y = (y * -1)
+  equivalence_wrt_operation_lemma #a #mul eq (neg y) (y `mul` neg one) x; // x*(-y) = x*(y*(-1))
+  associative_operation_lemma eq mul x y (neg one);                       // x*(y*(-1)) = (x*y)*(-1)
+  ring_additive_inv_x_is_x_times_minus_one r (x `mul` y);                 // (xy)*(-1) = -(xy)
+  trans_lemma eq (x `mul` neg y) (x `mul` (y `mul` neg one)) ((x `mul` y) `mul` neg one);
+  trans_lemma eq (x `mul` neg y) ((x `mul` y) `mul` neg one) (neg (x `mul` y));  
+  ()
+
+let ring_x_times_minus_y_is_minus_x_times_y (#a:Type) (r:ring #a) (x y: a) : Lemma (
+    (x `r.multiplication.op` r.addition.inv y) `r.eq` (r.addition.inv x `r.multiplication.op` y) &&
+    (r.addition.inv x `r.multiplication.op` y) `r.eq` (x `r.multiplication.op` r.addition.inv y) 
+  ) =   
+  let eq = r.eq in
+  let mul = r.multiplication.op in
+  let add = r.addition.op in
+  let neg = r.addition.inv in 
+  let zero = r.addition.neutral in
+  let one = r.multiplication.neutral in
+  ring_additive_inv_x_is_minus_one_times_x r y;  
+  associative_operation_lemma eq mul x (neg one) y;
+  assert (neg y `eq` mul (neg one) y);
+  equivalence_wrt_operation_lemma #a #mul eq (neg y) (mul (neg one) y) x;
+  assert ((x `mul` neg y) `eq` (x `mul` (neg one `mul` y)));
+  associative_operation_lemma eq mul x (neg one) y;
+  assert ((x `mul` (neg one `mul` y)) `eq` ((x `mul` neg one) `mul` y));
+  trans_lemma eq (x `mul` neg y) (x `mul` (neg one `mul` y)) ((x `mul` neg one) `mul` y);
+  assert (eq (x `mul` neg y) ((x `mul` neg one) `mul` y));
+  ring_additive_inv_x_is_x_times_minus_one r x;
+  assert ((x `mul` neg one) `eq` neg x);
+  equivalence_wrt_operation_lemma #a #mul eq (x `mul` neg one) (neg x) y;
+  assert ( ((x `mul` neg one) `mul` y) `eq` (neg x `mul` y) );
+  trans_lemma eq (x `mul` neg y) ((x `mul` neg one) `mul` y) (neg x `mul` y)
+
+let ring_product_with_minus_lemma (#a:Type) (r:ring #a) (x y: a) 
+  : Lemma (
+           (x `r.multiplication.op` r.addition.inv y) `r.eq` (r.addition.inv x `r.multiplication.op` y) /\
+           (x `r.multiplication.op` r.addition.inv y) `r.eq` (r.addition.inv (x `r.multiplication.op` y)) 
+          ) = 
+  ring_x_times_minus_y_is_minus_x_times_y r x y; 
+  ring_x_times_minus_y_is_minus_xy r x y 
+
+let neg_distr_lemma (#a:Type) (r: ring #a) (x y z: a) 
+  : Lemma ((x `r.multiplication.op` (y `r.addition.op` r.addition.inv z)) `r.eq` ((r.multiplication.op x y) `r.addition.op` (r.addition.inv (r.multiplication.op x z)))) =  
+  let eq = r.eq in
+  let mul = r.multiplication.op in
+  let add = r.addition.op in
+  let neg = r.addition.inv in 
+  let zero = r.addition.neutral in
+  let one = r.multiplication.neutral in
+  left_distributivity_lemma mul add eq x y (neg z);
+  ring_x_times_minus_y_is_minus_xy r x z;
+  assert ((x `mul` neg z) `eq` neg (x `mul` z)); 
+  equivalence_wrt_operation_lemma #a #add eq (x `mul` neg z) (neg (x `mul` z)) (x `mul` y);
+  assert (((x `mul` y) `add` (x `mul` neg z)) `eq` ((x `mul` y) `add` (neg (x `mul` z))));
+  trans_lemma eq (x `mul` (y `add` neg z)) ((x `mul` y) `add` (x `mul` neg z))  ((x `mul` y) `add` (neg (x `mul` z)));
+  ()
 
 let neut_add_lemma (#a: Type) (r: ring #a) : Lemma (is_neutral_of r.addition.neutral r.addition.op r.eq) = () 
 let neut_lemma (#a: Type) (r: ring #a) : Lemma (is_neutral_of r.multiplication.neutral r.multiplication.op r.eq) = ()
@@ -364,10 +719,21 @@ let is_zero_of (#a: Type) (r: ring #a) (x: a) = is_absorber_of x r.multiplicatio
 let two_zeros_are_equal (#a:Type) (r: ring #a) (x y: (t:a{r.eq t r.addition.neutral})) 
   : Lemma (x `r.eq` y) = ()
 
-let zero_is_equal_to_add_neutral_p (#a:Type) (r: ring #a) (z: a)
-  : Lemma (is_absorber_of z r.multiplication.op r.eq <==> r.eq z r.addition.neutral) 
-  =  () // let eq : equivalence_wrt r.addition.op = r.eq in neutral_is_unique r.addition r.addition.neutral z
+let eq_symmetry (#a:Type) (eq: equivalence_relation a) (x y: a) : Lemma (requires (x `eq` y \/ y `eq` x)) (ensures (x `eq` y /\ y `eq` x)) = ()
 
+#push-options "--ifuel 1 --fuel 0 --z3rlimit 2"
+let zero_is_equal_to_add_neutral_p (#a:Type) (r: ring #a) (z: a)
+  : Lemma (is_zero_of r z <==> r.eq z r.addition.neutral) 
+  =  
+  let eq = r.eq in
+  assert (is_absorber_of r.addition.neutral r.multiplication.op r.eq);
+  if (r.eq z r.addition.neutral) then 
+    absorber_equal_is_absorber r.multiplication.op r.eq r.addition.neutral z  
+  else (
+    FStar.Classical.move_requires_2 (absorber_is_unique r.multiplication.op r.eq) z r.addition.neutral;
+    assert_spinoff (is_absorber_of z r.multiplication.op r.eq <==> eq z r.addition.neutral) 
+  )
+#pop-options
 
 let zero_is_equal_to_add_neutral (#a:Type) (r: ring #a) : Lemma (forall (x:a). is_zero_of r x <==> r.eq x r.addition.neutral) 
   = FStar.Classical.forall_intro (zero_is_equal_to_add_neutral_p r)
@@ -378,17 +744,52 @@ let nonzero_is_equal_to_add_neutral (#a:Type) (r: ring #a)
 let nonzero_is_not_equal_to_add_neutral_p (#a:Type) (r: ring #a) (z: a)
   : Lemma (~(is_absorber_of z r.multiplication.op r.eq) <==> ~(r.eq z r.addition.neutral)) = zero_is_equal_to_add_neutral r
 
+
 type domain (#a: Type) = r:ring #a { has_no_absorber_divisors r.multiplication.op r.eq }
 
-let dom_prod_zero_lemma (#a:Type) (dom: domain #a) (p q: a) 
+ 
+#push-options "--ifuel 1 --fuel 0 --z3rlimit 2"
+private let domain_mul_absorber_lemma (#a:Type) (dom: domain #a) (x y:a) 
+  : Lemma (is_absorber_of (dom.multiplication.op x y) dom.multiplication.op dom.eq <==> 
+           is_absorber_of x dom.multiplication.op dom.eq \/ is_absorber_of y dom.multiplication.op dom.eq) = 
+   domain_multiplication_law_inv dom.eq dom.multiplication.op x y
+#pop-options
+
+
+private let domain_lemma_1 (#a:Type) (dom: domain #a) (p q:a) : Lemma (requires is_absorber_of p dom.multiplication.op dom.eq \/ is_absorber_of p dom.multiplication.op dom.eq)
+                                                              (ensures is_absorber_of (dom.multiplication.op p q) dom.multiplication.op dom.eq) = ()
+                                               
+private let domain_lemma_2 (#a:Type) (dom: domain #a) (x y:a) 
+  : Lemma (requires is_absorber_of (dom.multiplication.op x y) dom.multiplication.op dom.eq) 
+          (ensures is_absorber_of x dom.multiplication.op dom.eq \/ is_absorber_of y dom.multiplication.op dom.eq) = 
+  domain_mul_absorber_lemma dom x y
+ 
+let domain_zero_product_means_zero_factor (#a:Type) (dom: domain #a) (p q: a) 
   : Lemma (requires (p `dom.multiplication.op` q) `dom.eq` dom.addition.neutral)
           (ensures (p `dom.eq` dom.addition.neutral \/ q `dom.eq` dom.addition.neutral)) =     
-          let pq = p `dom.multiplication.op` q in
-          neutral_equivalent_is_neutral dom.addition.op dom.eq  dom.addition.neutral pq;
-          neutral_is_unique dom.addition dom.addition.neutral pq;
-          ()
+  neutral_equivalent_is_neutral dom.addition.op dom.eq dom.addition.neutral (p `dom.multiplication.op` q);
+  absorber_equal_is_absorber dom.multiplication.op dom.eq dom.addition.neutral (p `dom.multiplication.op` q); 
+  domain_multiplication_law_inv dom.eq dom.multiplication.op p q;
+  zero_is_equal_to_add_neutral dom
 
-
+#push-options "--ifuel 1 --fuel 0 --z3rlimit 1"
+let domain_characterizing_lemma (#a:Type) (dom: domain #a) (p q: a) 
+  : Lemma ((p `dom.multiplication.op` q) `dom.eq` dom.addition.neutral <==>
+           (p `dom.eq` dom.addition.neutral \/ q `dom.eq` dom.addition.neutral)) =     
+  FStar.Classical.move_requires_2 (domain_zero_product_means_zero_factor dom) p q;
+  if (dom.eq p dom.addition.neutral) then (
+    absorber_equal_is_absorber dom.multiplication.op dom.eq dom.addition.neutral p;
+    absorber_lemma dom.multiplication.op dom.eq p q;
+    assert (p `dom.multiplication.op` q `dom.eq` dom.addition.neutral);
+    ()
+  ) else if (dom.eq q dom.addition.neutral) then (
+    absorber_equal_is_absorber dom.multiplication.op dom.eq dom.addition.neutral q;
+    absorber_lemma dom.multiplication.op dom.eq q p;
+    assert (p `dom.multiplication.op` q `dom.eq` dom.addition.neutral);
+    ()
+  ) else ()
+#pop-options
+  
 type commutative_ring (#a: Type) = r:ring #a { is_commutative r.multiplication.op r.eq }
 
 /// I'm not 100% sure, but somehow I think that PERHAPS unit/normal part functions
@@ -401,12 +802,16 @@ type commutative_ring (#a: Type) = r:ring #a { is_commutative r.multiplication.o
 /// The special case of euclidean domains, which allows for reduced fractions, will be handled
 /// differently, and all arithmetics will also account for the gcd/eea availability.
 /// 
-type integral_domain (#a: Type) = r:domain #a { is_commutative r.multiplication.op r.eq }
+type integral_domain (#a: Type) = r:domain #a 
+{ 
+  is_commutative r.multiplication.op r.eq /\
+  is_unit_part_function r.unit_part_of /\
+  is_normal_part_function r.unit_part_of r.normal_part_of  
+  
+}
 
 type euclidean_domain (#a:Type) = r:integral_domain #a 
 { 
-  euclidean_norm_forall_property r.eq r.multiplication.op r.euclidean_norm /\
-  is_unit_part_function r.unit_part_of /\
-  is_normal_part_function r.unit_part_of r.normal_part_of  
+  euclidean_norm_forall_property r.eq r.multiplication.op r.euclidean_norm
 }
  
